src/core/DY.Core.Attacker.Knowledge.fst
@@ -165,7 +165,7 @@ let rec attacker_knows_aux step tr msg =
     // MAC
     (
       exists key buf.
-        msg == mac_auth key buf /\
+        msg == mac_compute key buf /\
         attacker_knows_aux (step-1) tr key /\
         attacker_knows_aux (step-1) tr buf
     )
@@ -234,7 +234,7 @@ let rec attacker_only_knows_publishable_values_aux #invs step tr msg =
     FStar.Classical.forall_intro   (FStar.Classical.move_requires   (kem_pk_preserves_publishability tr));
     FStar.Classical.forall_intro_2 (FStar.Classical.move_requires_2 (kem_encap_preserves_publishability tr));
     FStar.Classical.forall_intro_2 (FStar.Classical.move_requires_2 (kem_decap_preserves_publishability tr));
-    FStar.Classical.forall_intro_2 (FStar.Classical.move_requires_2 (mac_auth_preserves_publishability tr));
+    FStar.Classical.forall_intro_2 (FStar.Classical.move_requires_2 (mac_compute_preserves_publishability tr));
     ()
   )
 #pop-options
